Java/src/Java/Func/Reify.v
@@ -243,7 +243,6 @@ Goal (forall (Pr : Program) (C : class) (v : val) (fields : list field), True).
   intros Pr C v fields.
 
   reify_imp (typeof C v).
-
   reify_imp (field_lookup).
   reify_imp (field_lookup Pr C fields).
 
@@ -278,10 +277,10 @@ Goal (forall (Pr : Program) (C : class) (v : val) (fields : list field), True).
   reify_imp (forall x : nat, x = x).
   reify_imp (exists x : nat, x = x).
 
-  reify_imp (@map nat nat).
   reify_imp (@subst1 Lang.var val _).
   reify_imp (cseq cskip cskip).
 
+(*  reify_imp (@map nat nat).*)
   reify_imp (ILogic.lentails True True).
 
   reify_imp ((True -> False) -> True).
