Java/src/Java/Logic/SpecLogic.v
@@ -29,14 +29,16 @@ Definition mk_spec (f: Program -> nat -> Prop)
   (HSPred: forall k P P', Prog_sub P P' -> f P k -> f P' k) : spec.
   refine (mkILPreFrm (fun k => mkILPreFrm (f k) _) _).
 Proof.
-  + intros n m Hnk S'. generalize dependent m. induction n; intros.
+  + assert (forall k P P', Prog_sub P P' -> f P k -> f P' k) as HProg.
+    intros k' P P' HPP' S'. eapply HSPred; eassumption. 
+    intros p p' Hp'' n S'; simpl in *. eapply HProg; eassumption.
+  
+  Unshelve.
+      intros n m H1 S'. generalize dependent m. induction n; intros.
     - assert (m = 0) by omega; subst. apply S'.
     - destruct (gt_eq_gt_dec m (S n)) as [[H | H] | H]; [| | omega].
       * apply IHn. apply Hnat. apply S'. omega.
       * subst. apply S'.
-  + assert (forall k P P', Prog_sub P P' -> f P k -> f P' k) as HProg.
-    intros k' P P' HPP' S'. eapply HSPred; eassumption. 
-    intros p p' Hp'' n S'; simpl in *. eapply HProg; eassumption.
 Defined.
 
 Program Definition prog_spec (X : Program -> Prop) : spec :=
